codelib/CodeLib.lean
@@ -11,6 +11,7 @@ import CodeLib.RustStd.MemArray
 import CodeLib.RustStd.MemFillLoop
 import CodeLib.RustStd.MemCopyLoop
 import CodeLib.RustStd.UInt
+import CodeLib.RustStd.Option
 import CodeLib.RustStd.U64.Basic
 import CodeLib.RustStd.U64.AbsDiff
 import CodeLib.RustStd.U64.Add
